Fix issues after merge

src/lib/communication/DY.Lib.Communication.RequestResponse.Lemmas.fst
@@ -235,22 +235,43 @@ let receive_request_proof #invs #a #config tr comm_keys_ids higher_layer_preds s
     let req_msg_bytes:bytes = serialize comm_message_t req_msg_t in
     let req_send_event client:communication_reqres_event a = CommClientSendRequest client server request req_msg.key in
 
-    conf_message_secrecy tr' request_response_event_preconditions server req_msg_bytes;
+    conf_message_properties tr_recv (comm_core_higher_layer_event_preds_reqres a) server req_msg_t;
+    
+    // Properties that can be proved uniformly in both the honest and corrupt case
+    eliminate (exists client. event_triggered tr_recv client (req_send_event client)) \/
+              (is_publishable tr_recv req_msg.request /\ is_publishable tr_recv req_msg.key)
+    returns (
+      is_well_formed a (is_knowable_by (get_response_label tr_recv req_meta_data) tr_recv) request /\
+      req_msg.key `has_usage tr_recv` (AeadKey (comm_layer_aead_tag a) empty)
+    )
+    with _. eliminate exists client. event_triggered tr_recv client (req_send_event client)
+      returns _
+      with _. (
+        get_response_label_eq_key_label tr_recv req_meta_data;
 
-    assert(is_knowable_by (get_label tr' req_msg.key) tr' req_msg.request);
-    FStar.Classical.move_requires (has_usage_publishable tr' req_msg.key) (AeadKey comm_layer_aead_tag empty);
-    assert(req_msg.key `has_usage tr'` (AeadKey comm_layer_aead_tag empty));
+        let i = find_event_triggered_at_timestamp tr_recv client (req_send_event client) in
+        assert(event_predicate_communication_layer_reqres higher_layer_preds (prefix tr_recv i) client (req_send_event client));
+        ()
+      )
+    and _. (has_usage_publishable tr_recv req_msg.key (AeadKey (comm_layer_aead_tag a) empty);
+      parse_wf_lemma a (is_publishable tr_recv) req_msg.request;
+      ()
+    );
 
     // Relating knowledge of the request to knowledge of its fields
     serialize_parse_inv_lemma #bytes a req_msg.request;
-    let Some payload' = parse a req_msg.request in
-    assert(is_comm_response_payload tr' server req_meta_data payload');
+    assert(is_comm_response_payload tr_recv server req_meta_data payload);
 
-    let ((), tr') = trigger_event server (CommServerReceiveRequest server req_msg.request req_msg.key) tr' in
-    assert(trace_invariant tr');
-    let (sid', tr') = new_session_id server tr' in
-    let ((), tr') = set_state server sid' (ServerReceiveRequest {request=req_msg.request; key=req_msg.key} <: communication_states) tr' in
-    assert(tr' == tr_out);
+    let ((), tr_ev) = trigger_event server (CommServerReceiveRequest server request req_msg.key <: communication_reqres_event a) tr_recv in
+    let (sid', tr_sess) = new_session_id server tr_ev in
+
+    // Needed for the proof to go through
+    assert((state_predicate_communication_layer_reqres a).pred tr_sess server sid' (ServerReceiveRequest {request; key=req_msg.key} <: communication_states a));
+    let ((), tr_st) = set_state server sid' (ServerReceiveRequest {request; key=req_msg.key} <: communication_states a) tr_sess in
+
+    get_response_label_eq_key_label tr_recv req_meta_data;
+    
+    assert(tr_out == tr_st);
     assert(trace_invariant tr_out);
     ()
   )
@@ -345,7 +366,6 @@ let compute_response_message_proof #cinvs #a tr server req_meta_data nonce reque
   FStar.Classical.move_requires (aead_enc_preserves_publishability tr req_meta_data.key nonce res_bytes) ad_bytes;
   serialize_wf_lemma comm_message_t (is_publishable tr) (ResponseMessage {nonce; ciphertext});
   ()
-#pop-options
 
 #push-options "--z3rlimit 10"
 val send_response_proof:
@@ -389,7 +409,6 @@ let send_response_proof #invs #a tr higher_layer_preds server req_meta_data resp
     assert(trace_invariant tr_out); 
     ()
   )
-#pop-options
 #pop-options
 
 
